Tweak clos_callProof statement again
After chat with Magnus and Michael, the new version uses a "fixed,
late" g1 and l1 (compiler state) in the inductive hypothesis, to avoid
too much dependence on the exact relationship to the compiler
invocation. This commit recovers previous progress (Fn and App cases
work), but now the evaluate_app case looks more plausible (at a glance
at least)...

compiler/backend/proofs/clos_callProofScript.sml
@@ -121,15 +121,21 @@ val v_rel_def = tDefine"v_rel"`
   (v_rel g l (Closure loco vs1 env1 n bod1) v ⇔
      ∃g0 l0 vs2 env2.
        closure_rel g l g0 l0 (Closure loco vs1 env1 n bod1) v vs2 env2 ∧
-       LIST_REL (v_rel g l) vs1 vs2 ∧ LIST_REL (v_rel g0 l0) env1 env2) ∧
+       LIST_REL (v_rel g l) vs1 vs2 ∧ LIST_REL (v_rel g l) env1 env2) ∧
   (v_rel g l (Recclosure loco vs1 env1 fns1 i) v ⇔
      ∃g0 l0 vs2 env2.
        recclosure_rel g l g0 l0 (Recclosure loco vs1 env1 fns1 i) v vs2 env2 ∧
-       LIST_REL (v_rel g l) vs1 vs2 ∧ LIST_REL (v_rel g0 l0) env1 env2)`
+       LIST_REL (v_rel g l) vs1 vs2 ∧ LIST_REL (v_rel g l) env1 env2)`
   (WF_REL_TAC `measure (v_size o FST o SND o SND)` >> simp[v_size_def] >>
    rpt strip_tac >> imp_res_tac v_size_lemma >> simp[]);
 
 val v_rel_ind = theorem"v_rel_ind";
+
+val clos_rel_def = Define`
+  clos_rel g l g0 l0 v1 v2 ⇔
+    ∃vs2 env2.
+      closure_rel g l g0 l0 v1 v2 vs2 env2 ∨
+      recclosure_rel g l g0 l0 v1 v2 vs2 env2`;
 
 val code_includes_def = Define`
   code_includes al code ⇔
@@ -495,7 +501,7 @@ val v_rel_subg = Q.store_thm("v_rel_subg",
     \\ qpat_assum`LIST_REL (v_rel g l) l1 l2` kall_tac
     \\ map_every qunabbrev_tac[`l2`,`l1`])
   \\ fs[]
-  \\ qexists_tac`g0`
+  \\ qexists_tac`g0` \\ qexists_tac`l0`
   \\ rpt(pairarg_tac \\ fs[])
   \\ IF_CASES_TAC \\ fs[]
   \\ metis_tac[subg_trans,SUBSET_DEF]);
@@ -620,6 +626,24 @@ val v_rel_min = Q.store_thm("v_rel_min",
     \\ fs[subg_def]
 *)
 
+(*
+val evaluate_app_imp_clos_rel = Q.store_thm("evaluate_app_imp_clos_rel",
+  `evaluate_app loco v args s = (res,s') ∧
+   v_rel g l v v' ∧ args ≠ [] ∧
+   res ≠ Rerr (Rabort Rtype_error)
+   ⇒
+   ∃g0 l0. clos_rel g l g0 l0 v v'`,
+  rw[]
+  \\ fs[evaluate_app_rw]
+  \\ last_x_assum mp_tac
+  \\ BasicProvers.TOP_CASE_TAC \\ fs[]
+  \\ fs[dest_closure_def]
+  \\ pop_assum mp_tac
+  \\ BasicProvers.TOP_CASE_TAC \\ fs[]
+  \\ fs[v_rel_def,clos_rel_def]
+  \\ metis_tac[]);
+*)
+
 val dest_closure_v_rel_lookup = Q.store_thm("dest_closure_v_rel_lookup",
   `dest_closure (SOME loc) v1 env1 = SOME x ∧
    v_rel g l v1 v2 ∧
@@ -657,6 +681,7 @@ val dest_closure_v_rel_lookup = Q.store_thm("dest_closure_v_rel_lookup",
       \\ rfs[ALL_DISTINCT_APPEND,MEM_MAP,PULL_EXISTS]
       \\ res_tac \\ fs[] )
     \\ fsrw_tac[ETA_ss][]
+    (*
     \\ `subg g0 g`
     by (
       qpat_assum`calls _ (insert_each _ _ _) = _`assume_tac
@@ -678,7 +703,8 @@ val dest_closure_v_rel_lookup = Q.store_thm("dest_closure_v_rel_lookup",
       \\ rfs[SUBSET_DEF]
       \\ fs[ALL_DISTINCT_APPEND] )
     \\ match_mp_tac (GEN_ALL (MP_CANON LIST_REL_mono))
-    \\ metis_tac[v_rel_subg])
+    \\ metis_tac[v_rel_subg]
+    *))
   \\ last_assum(part_match_exists_tac(el 2 o strip_conj) o concl)
   \\ asm_exists_tac \\ simp[]
   \\ qhdtm_x_assum`COND`mp_tac
@@ -720,6 +746,7 @@ val dest_closure_v_rel_lookup = Q.store_thm("dest_closure_v_rel_lookup",
   \\ simp[v_rel_def,recclosure_rel_def]
   \\ fsrw_tac[ETA_ss][]
   \\ simp[calls_list_MAPi]
+  (*
   \\ reverse conj_tac
   >- (
     `subg g0 g`
@@ -752,6 +779,7 @@ val dest_closure_v_rel_lookup = Q.store_thm("dest_closure_v_rel_lookup",
       \\ metis_tac[ADD_ASSOC,ADD1,numTheory.INV_SUC])
     \\ match_mp_tac (GEN_ALL (MP_CANON LIST_REL_mono))
     \\ metis_tac[v_rel_subg])
+  *)
   \\ rw[]
   \\ qexists_tac`g0`
   \\ qexists_tac`l0''`
@@ -770,9 +798,7 @@ val dest_closure_v_rel = Q.store_thm("dest_closure_v_rel",
       ∃e2 args2 rest2.
         x2 = Full_app e2 args2 rest2 ∧
         LIST_REL (v_rel g l) args1 args2 ∧
-        (*
         LIST_REL (v_rel g l) rest1 rest2 ∧
-        *) LENGTH rest1 = LENGTH rest2 ∧
         every_Fn_SOME [e1] ∧
         every_Fn_vs_NONE [e1] ∧
         set (code_locs [e1]) ⊆ EVEN ∧
@@ -785,16 +811,13 @@ val dest_closure_v_rel = Q.store_thm("dest_closure_v_rel",
   \\ rpt(pairarg_tac \\ fs[])
   >- (
     fs[revtakerev,revdroprev]
-    (* \\ conj_tac *)
+    \\ conj_tac
     >- (
       match_mp_tac EVERY2_APPEND_suff
       \\ fsrw_tac[ETA_ss][]
-      \\ conj_tac
-      >- (
-        match_mp_tac EVERY2_APPEND_suff \\ fs[]
-        \\ match_mp_tac EVERY2_DROP \\ fs[] )
-      \\ cheat)
-    (* \\ match_mp_tac EVERY2_TAKE \\ fs[] *))
+      \\ match_mp_tac EVERY2_APPEND_suff \\ fs[]
+      \\ match_mp_tac EVERY2_DROP \\ fs[] )
+    \\ match_mp_tac EVERY2_TAKE \\ fs[])
   >- (
     simp[v_rel_def,closure_rel_def]
     \\ qexists_tac`g0` \\ qexists_tac`l0'` \\ fs[]
@@ -818,7 +841,7 @@ val dest_closure_v_rel = Q.store_thm("dest_closure_v_rel",
   \\ conj_tac
   >- (
     match_mp_tac EVERY2_APPEND_suff \\ fs[]
-    \\ reverse conj_tac >- cheat
+    (* \\ reverse conj_tac >- cheat *)
     \\ match_mp_tac EVERY2_APPEND_suff
     \\ fs[LIST_REL_GENLIST]
     \\ conj_tac
@@ -829,10 +852,8 @@ val dest_closure_v_rel = Q.store_thm("dest_closure_v_rel",
     \\ ntac 2 strip_tac
     \\ qexists_tac`g0` \\ qexists_tac`l0'`
     \\ fsrw_tac[ETA_ss][] )
-  (*
   \\ conj_tac
   >- ( match_mp_tac EVERY2_TAKE \\ fs[] )
-  *)
   \\ fs[Q.SPEC`MAP _ _`every_Fn_SOME_EVERY,
         Q.SPEC`MAP _ _`every_Fn_vs_NONE_EVERY,
         code_locs_map,
@@ -854,7 +875,7 @@ val dest_closure_v_rel = Q.store_thm("dest_closure_v_rel",
 (* compiler correctness *)
 
 val calls_correct = Q.store_thm("calls_correct",
-  `(∀tmp xs env1 (s0:'ffi closSem$state) g0 g env2 t0 ys res s l0 l.
+  `(∀tmp xs env1 (s0:'ffi closSem$state) g0 g env2 t0 ys res s l0 l l1 g1.
     tmp = (xs,env1,s0) ∧
     evaluate (xs,env1,s0) = (res,s) ∧
     res ≠ Rerr (Rabort Rtype_error) ∧
@@ -864,21 +885,40 @@ val calls_correct = Q.store_thm("calls_correct",
     wfg g0 ∧
     ALL_DISTINCT (code_locs xs) ∧
     DISJOINT (IMAGE SUC (set (code_locs xs))) (set (MAP FST (SND g0))) ∧
-    LIST_REL (v_rel g0 l0) env1 env2 ∧
     DISJOINT l0 (domain (FST g0)) ∧ DISJOINT l0 (set (code_locs xs)) ∧
     l = l0 ∪ (set (code_locs xs) DIFF domain (FST g)) ∧
-    state_rel g0 l0 s0 t0 ∧ code_includes (SND g) t0.code
+    (*
+    LIST_REL (v_rel g0 l0) env1 env2 ∧
+    state_rel g0 l0 s0 t0 ∧
+    *)
+    (*
+    LIST_REL (v_rel g l) env1 env2 ∧
+    state_rel g l s0 t0 ∧
+    *)
+    LIST_REL (v_rel g1 l1) env1 env2 ∧
+    state_rel g1 l1 s0 t0 ∧
+    subg g g1 ∧ l ⊆ l1 ∧ DISJOINT l1 (domain (FST g1)) ∧ wfg g1 ∧
+    (*
+    subg g0 g1 ∧ subg g1 g ∧ l0 ⊆ l1 ∧ l1 ⊆ l
+    ∧ l = l0 ∪ (set (code_locs xs) DIFF domain (FST g)) ∧
+    *)
+    code_includes (SND g) t0.code
     ⇒
     ∃ck res' t.
     evaluate (ys,env2,t0 with clock := t0.clock + ck) = (res',t) ∧
-    state_rel g l s t ∧
-    result_rel (LIST_REL (v_rel g l)) (v_rel g l) res res') ∧
-  (∀loco f args (s0:'ffi closSem$state) loc g l t0 res s f' args'.
+    state_rel g1 l1 s t ∧
+    result_rel (LIST_REL (v_rel g1 l1)) (v_rel g1 l1) res res') ∧
+  (∀loco f args (s0:'ffi closSem$state) loc g l (* g0 l0 *) t0 res s f' args'.
     evaluate_app loco f args s0 = (res,s) ∧
     res ≠ Rerr (Rabort Rtype_error) ∧
     v_rel g l f f' ∧
     LIST_REL (v_rel g l) args args' ∧
     state_rel g l s0 t0
+    (*
+    clos_rel g l g0 l0 f f' ∧
+    LIST_REL (v_rel g0 l0) args args' ∧
+    state_rel g0 l0 s0 t0
+    *)
     ⇒
     ∃ck res' t.
     evaluate_app loco f' args' (t0 with clock := t0.clock + ck) = (res',t) ∧
@@ -891,10 +931,11 @@ val calls_correct = Q.store_thm("calls_correct",
     \\ qexists_tac`0`
     \\ fs[calls_def,evaluate_def]
     \\ rveq \\ fs[evaluate_def]
-    \\ simp[code_locs_def]
-    \\ metis_tac[state_rel_subg])
+    \\ fs[code_locs_def]
+    \\ metis_tac[state_rel_subg,SUBSET_REFL])
   \\ conj_tac
-  >- (
+  >- (cheat)
+  (*
     rw[evaluate_def,calls_def]
     \\ pairarg_tac \\ fs[]
     \\ pairarg_tac \\ fs[] \\ rveq
@@ -914,6 +955,7 @@ val calls_correct = Q.store_thm("calls_correct",
     \\ imp_res_tac calls_length
     \\ fs[quantHeuristicsTheory.LIST_LENGTH_2]
     \\ cheat )
+    *)
   (* Var *)
   \\ conj_tac >- cheat
   (* If *)
@@ -957,8 +999,8 @@ val calls_correct = Q.store_thm("calls_correct",
       \\ (impl_tac >- (fs[ALL_DISTINCT_APPEND] \\ fs[wfg_def]))
       \\ strip_tac \\ fs[]
       \\ match_mp_tac subg_trans
-      \\ last_assum (part_match_exists_tac (hd o strip_conj) o concl)
-      \\ simp[]
+      \\ qpat_assum`subg g0 (insert_each _ _ _)`assume_tac
+      \\ asm_exists_tac \\ rw[]
       \\ match_mp_tac subg_trans
       \\ asm_exists_tac \\ simp[]
       \\ fs[subg_def]
@@ -967,9 +1009,11 @@ val calls_correct = Q.store_thm("calls_correct",
       \\ rfs[SUBSET_DEF]
       \\ fs[ALL_DISTINCT_APPEND]
       \\ metis_tac[numTheory.INV_SUC] )
+    (*
     \\ qpat_abbrev_tac`l = l0 ∪ _`
     \\ `l0 ⊆ l` by simp[Abbr`l`]
     \\ `state_rel g l s t0` by metis_tac[state_rel_subg]
+    *)
     \\ `subspt (FST g0) (FST g)` by fs[subg_def]
     \\ CONV_TAC(RESORT_EXISTS_CONV(sort_vars["l0'","g0'"]))
     \\ qexists_tac`l0` \\ qexists_tac`g0` \\ fs[]
@@ -1014,11 +1058,24 @@ val calls_correct = Q.store_thm("calls_correct",
     \\ fs[DISJOINT_SYM]
     \\ imp_res_tac calls_add_SUC_code_locs
     \\ fs[SUBSET_DEF,GSYM ADD1]
+    \\ first_x_assum match_mp_tac
+    \\ rfs[wfg_def,PULL_EXISTS]
+    \\ metis_tac[]
+    (*
     \\ rpt conj_tac
+    \\ TRY (
+      match_mp_tac (GEN_ALL state_rel_subg) \\ fs[]
+      \\ first_assum(part_match_exists_tac (el 2 o strip_conj) o concl)
+      \\ simp[] )
     \\ TRY ( match_mp_tac subg_refl \\ fs[wfg_def] )
+    \\ TRY (
+      match_mp_tac (GEN_ALL (MP_CANON LIST_REL_mono))
+      \\ first_assum(part_match_exists_tac (last o strip_conj) o concl)
+      \\ metis_tac[v_rel_subg,SUBSET_DEF] )
     \\ strip_tac
     \\ `MEM (SUC x) (MAP FST (SND g))` by fs[wfg_def]
     \\ metis_tac[numTheory.INV_SUC]
+    *)
     (*
     \\ TRY ( reverse conj_tac >- (
       TRY (
@@ -1039,7 +1096,7 @@ val calls_correct = Q.store_thm("calls_correct",
       \\ match_mp_tac subg_refl \\ fs[subg_def] ))
     \\ match_mp_tac (GEN_ALL (MP_CANON LIST_REL_mono))
     \\ first_assum(part_match_exists_tac (last o strip_conj) o concl)
-    \\ metis_tac[v_rel_subg]
+    \\ metis_tac[v_rel_subg,SUBSET_REFL]
     *)
     )
   (* Letrec *)
@@ -1063,8 +1120,10 @@ val calls_correct = Q.store_thm("calls_correct",
     \\ strip_tac
     \\ `g'' = g` by (every_case_tac \\ fs[])
     \\ rveq \\ fs[]
+    (*
     \\ qpat_abbrev_tac`l = l0 ∪ _`
     \\ `l0 ⊆ l` by simp[Abbr`l`]
+    *)
     \\ `wfg g'`
     by (
       match_mp_tac calls_wfg
@@ -1079,7 +1138,21 @@ val calls_correct = Q.store_thm("calls_correct",
       strip_tac \\ rveq \\ rfs[]
       \\ first_x_assum drule \\ fs[DISJOINT_SYM,ALL_DISTINCT_APPEND]
       \\ rpt(disch_then drule)
-      \\ impl_tac >- ( metis_tac[code_includes_subg] )
+      \\ impl_tac
+      >- (
+        conj_tac >- metis_tac[subg_trans]
+        \\ simp[]
+        \\ reverse conj_tac >- metis_tac[code_includes_subg]
+        \\ fs[SUBSET_DEF]
+        \\ fs[subg_def]
+        \\ imp_res_tac subspt_domain_SUBSET
+        \\ fs[SUBSET_DEF] \\ rw[]
+        \\ Cases_on`x ∉ domain (FST g)` >- metis_tac[]
+        \\ fs[]
+        \\ imp_res_tac calls_add_SUC_code_locs
+        \\ rfs[wfg_def,SUBSET_DEF,PULL_EXISTS]
+        \\ metis_tac[])
+      (*
       \\ qpat_abbrev_tac`l' = l0 ∪ _`
       \\ `l' ⊆ l`
       by (
@@ -1091,14 +1164,23 @@ val calls_correct = Q.store_thm("calls_correct",
         \\ `¬MEM (SUC x) (MAP FST (SND g'))` by ( fs[wfg_def] )
         \\ fs[SUBSET_DEF]
         \\ metis_tac[numTheory.INV_SUC] )
+      \\ rfs[]
+      \\ disch_then(qspecl_then[`env2`,`t0`,`g'`]mp_tac)
+      \\ impl_tac
+      >- (
+        conj_tac
+        >- (
+          match_mp_tac (GEN_ALL (MP_CANON LIST_REL_mono))
+          \\ metis_tac[v_rel_subg]
+      *)
       \\ strip_tac
       \\ qexists_tac`ck`
       \\ imp_res_tac calls_length
-      \\ `state_rel g l r t`
+      \\ `state_rel g1 l1 r t`
       by (
         imp_res_tac evaluate_const \\ fs[]
         \\ metis_tac[state_rel_subg] )
-      \\ `exc_rel (v_rel g l) e e'`
+      \\ `exc_rel (v_rel g1 l1) e e'`
       by ( Cases_on`e`\\fs[] \\ metis_tac[v_rel_subg])
       \\ every_case_tac \\ fs[] \\ rw[evaluate_def]
       \\ simp[evaluate_append])
@@ -1109,8 +1191,22 @@ val calls_correct = Q.store_thm("calls_correct",
     \\ first_x_assum drule \\ fs[DISJOINT_SYM]
     \\ fs[ALL_DISTINCT_APPEND]
     \\ rpt(disch_then drule)
-    \\ impl_tac >- metis_tac[code_includes_subg]
+    \\ impl_tac
+    >- (
+      conj_tac >- metis_tac[subg_trans]
+      \\ simp[]
+      \\ reverse conj_tac >- metis_tac[code_includes_subg]
+      \\ fs[SUBSET_DEF]
+      \\ fs[subg_def]
+      \\ imp_res_tac subspt_domain_SUBSET
+      \\ fs[SUBSET_DEF] \\ rw[]
+      \\ Cases_on`x ∉ domain (FST g)` >- metis_tac[]
+      \\ fs[]
+      \\ imp_res_tac calls_add_SUC_code_locs
+      \\ rfs[wfg_def,SUBSET_DEF,PULL_EXISTS]
+      \\ metis_tac[])
     \\ strip_tac \\ fs[]
+    (*
     \\ qmatch_asmsub_abbrev_tac`v_rel g' l'`
     \\ `l' ⊆ l`
     by (
@@ -1122,11 +1218,14 @@ val calls_correct = Q.store_thm("calls_correct",
       \\ `¬MEM (SUC x) (MAP FST (SND g'))` by ( fs[wfg_def])
       \\ fs[SUBSET_DEF]
       \\ metis_tac[numTheory.INV_SUC] )
-    \\ disch_then(qspecl_then[`env2`,`t`,`l'`]mp_tac)
-    \\ `DISJOINT l' (domain (FST g'))`
+    *)
+    \\ disch_then(qspecl_then[`env2`,`t`,`l0`]mp_tac)
+    \\ `DISJOINT l0 (domain (FST g'))`
     by (
-      fs[Abbr`l'`,IN_DISJOINT]
+      fs[IN_DISJOINT]
+      (*
       \\ reverse conj_tac >- metis_tac[]
+      *)
       \\ spose_not_then strip_assume_tac
       \\ `x ∉ domain (FST g0)` by metis_tac[]
       \\ `¬MEM (SUC x) (MAP FST (SND g0))` by fs[wfg_def]
@@ -1137,19 +1236,24 @@ val calls_correct = Q.store_thm("calls_correct",
         \\ fs[SUBSET_DEF]
         \\ metis_tac[numTheory.INV_SUC])
       \\ metis_tac[])
-    \\ `DISJOINT l' (set (code_locs [x1]))`
+    \\ `DISJOINT l0 (set (code_locs [x1]))`
     by (
-      fs[Abbr`l'`,IN_DISJOINT]
+      fs[IN_DISJOINT]
       \\ spose_not_then strip_assume_tac
       \\ fs[ALL_DISTINCT_APPEND]
       \\ metis_tac[] )
-    \\ `l0 ⊆ l'` by simp[Abbr`l'`]
+    (* \\ `l0 ⊆ l'` by simp[Abbr`l'`] *)
+    \\ disch_then(qspecl_then[`l1`,`g1`]mp_tac)
     \\ impl_tac
     >- (
       imp_res_tac evaluate_const \\ fs[]
+      (*
       \\ match_mp_tac (GEN_ALL (MP_CANON LIST_REL_mono))
-      \\ metis_tac[v_rel_subg,subg_trans] )
+      \\ metis_tac[v_rel_subg,subg_trans]
+      *)
+      \\ fs[SUBSET_DEF])
     \\ strip_tac \\ rveq
+    (*
     \\ qmatch_assum_abbrev_tac`state_rel g ll _ _`
     \\ `ll ⊆ l`
     by ( simp[Abbr`ll`,Abbr`l`,SUBSET_DEF] )
@@ -1159,6 +1263,7 @@ val calls_correct = Q.store_thm("calls_correct",
       match_mp_tac subg_refl
       \\ imp_res_tac calls_ALL_DISTINCT
       \\ rfs[DISJOINT_SYM] )
+    *)
     \\ qpat_assum`_ = (ys,_)`mp_tac
     \\ qmatch_goalsub_abbrev_tac`COND b`
     \\ reverse IF_CASES_TAC \\ fs[]
@@ -1175,17 +1280,26 @@ val calls_correct = Q.store_thm("calls_correct",
         \\ qpat_assum`evaluate(es,env2,_) = _`(mp_tac o MATCH_MP evaluate_add_clock)
         \\ disch_then(qspec_then`ck'`mp_tac) \\ simp[] \\ strip_tac
         \\ qexists_tac`ck+ck'` \\ fs[]
+        (*
         \\ imp_res_tac evaluate_const \\ fs[]
         \\ conj_tac >- metis_tac[state_rel_subg]
         \\ Cases_on`e` \\ fs[]
-        \\ metis_tac[v_rel_subg])
+        \\ metis_tac[v_rel_subg]*))
       \\ strip_tac \\ fs[] \\ rfs[]
       \\ imp_res_tac evaluate_length_imp
       \\ fs[quantHeuristicsTheory.LIST_LENGTH_2]
       \\ rveq \\ fs[]
+      (*
+      \\ drule (GEN_ALL evaluate_app_imp_clos_rel)
+      \\ disch_then drule
+      \\ impl_tac >- (CCONTR_TAC \\ fs[] \\ fs[])
+      \\ strip_tac
+      *)
       \\ first_x_assum drule
+      (*
       \\ qmatch_assum_rename_tac `LIST_REL (v_rel g' l') ev1 ev2`
       \\ `LIST_REL (v_rel g ll) ev1 ev2` by metis_tac[LIST_REL_mono,v_rel_subg]
+      *)
       \\ disch_then drule
       \\ disch_then drule
       \\ strip_tac \\ simp[]
@@ -1194,14 +1308,21 @@ val calls_correct = Q.store_thm("calls_correct",
       \\ qpat_assum`evaluate([_],env2,_) = _`(mp_tac o MATCH_MP evaluate_add_clock)
       \\ disch_then(qspec_then`ck''`mp_tac) \\ simp[] \\ strip_tac
       \\ qexists_tac`ck+ck'+ck''` \\ fs[]
+      (*
       \\ conj_tac >- metis_tac[state_rel_subg,state_rel_def]
       \\ Cases_on`res` \\ fs[] \\ TRY (Cases_on`e` \\ fs[])
       \\ TRY (match_mp_tac (GEN_ALL (MP_CANON LIST_REL_mono)))
-      \\ metis_tac[v_rel_subg])
+      \\ metis_tac[v_rel_subg]*))
     \\ qpat_assum`Abbrev(IS_SOME _ ∧ _)`mp_tac
     \\ simp[markerTheory.Abbrev_def,IS_SOME_EXISTS]
     \\ strip_tac \\ rveq \\ fs[]
     \\ `x ∈ domain (FST g)` by simp[domain_lookup]
+    \\ `x ∈ domain (FST g1)` by (
+      fs[subg_def]
+      \\ imp_res_tac subspt_domain_SUBSET
+      \\ fs[SUBSET_DEF] )
+    \\ `x ∉ l1` by ( fs[IN_DISJOINT] \\ metis_tac[] )
+    (*
     \\ `x ∉ ll`
     by (
       simp[Abbr`ll`]
@@ -1218,6 +1339,7 @@ val calls_correct = Q.store_thm("calls_correct",
       \\ `x ∉ l0` by (fs[IN_DISJOINT] \\ metis_tac[])
       \\ simp[Abbr`l'`]
       \\ fs[ALL_DISTINCT_APPEND] )
+    *)
     \\ IF_CASES_TAC \\ fs[] \\ strip_tac \\ rveq \\ fs[]
     \\ simp[evaluate_def]
     >- (
@@ -1229,8 +1351,11 @@ val calls_correct = Q.store_thm("calls_correct",
       \\ ntac 2 strip_tac \\ rveq
       \\ fs[quantHeuristicsTheory.LIST_LENGTH_2] \\ rveq
       \\ rfs[] \\ rveq
+      (*
       \\ qmatch_assum_rename_tac `LIST_REL (v_rel g' l') ev1 ev2`
       \\ `LIST_REL (v_rel g ll) ev1 ev2` by metis_tac[LIST_REL_mono,v_rel_subg]
+      *)
+      \\ qmatch_assum_rename_tac`LIST_REL (v_rel g1 l1) ev1 ev2`
       \\ Cases_on`ev1 = []`
       \\ imp_res_tac evaluate_length_imp \\ rfs[]
       \\ fs[evaluate_app_rw]
@@ -1242,12 +1367,31 @@ val calls_correct = Q.store_thm("calls_correct",
       \\ disch_then drule
       \\ impl_tac >- rw[]
       \\ strip_tac
+      \\ `ALOOKUP (SND g) (x+1) = ALOOKUP (SND g1) (x+1)`
+      by (
+        `ALL_DISTINCT (MAP FST (SND g1))` by fs[subg_def]
+        \\ `∃ls. SND g1 =  ls ++ SND g` by (metis_tac[subg_def,IS_SUFFIX_APPEND])
+        \\ pop_assum SUBST_ALL_TAC
+        \\ simp_tac(srw_ss())[ALOOKUP_APPEND]
+        \\ BasicProvers.CASE_TAC
+        \\ fs[ALL_DISTINCT_APPEND]
+        \\ imp_res_tac ALOOKUP_MEM
+        \\ `¬MEM (x+1) (MAP FST (SND g))`
+        by (
+          first_x_assum match_mp_tac
+          \\ simp[MEM_MAP,PULL_EXISTS]
+          \\ metis_tac[FST] )
+        \\ rfs[wfg_def,GSYM ADD1] )
+      \\ rfs[]
       \\ drule (GEN_ALL code_includes_ALOOKUP)
       \\ disch_then drule \\ strip_tac
       \\ `t.code = t0.code` by (imp_res_tac evaluate_const \\ fs[])
       \\ first_x_assum drule
       \\ disch_then drule
+      \\ qpat_assum`state_rel g1 l1 r t`assume_tac
+      (*
       \\ `state_rel g ll r t` by ( metis_tac[state_rel_subg] )
+      *)
       \\ disch_then drule
       \\ strip_tac
       \\ imp_res_tac LIST_REL_LENGTH \\ fs[]
@@ -1274,9 +1418,7 @@ val calls_correct = Q.store_thm("calls_correct",
         \\ `t'.clock = LENGTH ev2 - ck''` by decide_tac
         \\ fs[]
         \\ qexists_tac`ck` \\ simp[]
-        \\ fs[dec_clock_def]
-        \\ match_mp_tac (GEN_ALL state_rel_subg)
-        \\ fs[] \\ metis_tac[] )
+        \\ fs[dec_clock_def])
       \\ fs[NOT_LESS_EQUAL]
       \\ strip_tac
       \\ fs[dec_clock_def,TAKE_APPEND1]
@@ -1318,8 +1460,11 @@ val calls_correct = Q.store_thm("calls_correct",
     \\ qpat_assum`LENGTH [_] = _`(assume_tac o SYM) \\ fs[]
     \\ fs[quantHeuristicsTheory.LIST_LENGTH_2] \\ rveq \\ fs[] \\ rveq
     \\ first_x_assum drule
+    (*
     \\ qmatch_assum_rename_tac `LIST_REL (v_rel g' l') ev1 ev2`
     \\ `LIST_REL (v_rel g ll) ev1 ev2` by metis_tac[LIST_REL_mono,v_rel_subg]
+    *)
+    \\ qmatch_assum_rename_tac`LIST_REL (v_rel _ _) ev1 ev2`
     \\ rpt(disch_then drule)
     \\ strip_tac
     \\ simp[find_code_def]
@@ -1339,6 +1484,22 @@ val calls_correct = Q.store_thm("calls_correct",
     \\ qpat_assum`_ = (res',_)`mp_tac
     \\ imp_res_tac state_rel_clock \\ fs[]
     \\ imp_res_tac LIST_REL_LENGTH \\ fs[]
+    \\ `ALOOKUP (SND g) (x+1) = ALOOKUP (SND g1) (x+1)`
+    by (
+      `ALL_DISTINCT (MAP FST (SND g1))` by fs[subg_def]
+      \\ `∃ls. SND g1 =  ls ++ SND g` by (metis_tac[subg_def,IS_SUFFIX_APPEND])
+      \\ pop_assum SUBST_ALL_TAC
+      \\ simp_tac(srw_ss())[ALOOKUP_APPEND]
+      \\ BasicProvers.CASE_TAC
+      \\ fs[ALL_DISTINCT_APPEND]
+      \\ imp_res_tac ALOOKUP_MEM
+      \\ `¬MEM (x+1) (MAP FST (SND g))`
+      by (
+        first_x_assum match_mp_tac
+        \\ simp[MEM_MAP,PULL_EXISTS]
+        \\ metis_tac[FST] )
+      \\ rfs[wfg_def,GSYM ADD1] )
+    \\ rfs[]
     \\ imp_res_tac code_includes_ALOOKUP \\ fs[]
     \\ IF_CASES_TAC \\ fs[]
     >- (
@@ -1349,6 +1510,7 @@ val calls_correct = Q.store_thm("calls_correct",
       \\ qexists_tac`ck+ck'` \\ simp[]
       \\ match_mp_tac state_rel_with_clock
       \\ metis_tac[state_rel_subg])
+    \\ simp[Once dec_clock_def]
     \\ simp[evaluate_def,evaluate_GENLIST_Var]
     \\ simp[find_code_def]
     \\ simp[Once dec_clock_def]
@@ -1418,8 +1580,7 @@ val calls_correct = Q.store_thm("calls_correct",
     \\ first_x_assum drule
     \\ fs[code_locs_def]
     \\ disch_then drule \\ fs[]
-    \\ disch_then drule
-    \\ rw[]
+    \\ rpt(disch_then drule) \\ rw[]
     \\ qexists_tac`ck`
     \\ rw[] )
   \\ conj_tac >- ( rw[evaluate_def] \\ qexists_tac`0` \\ rw[] )
